theories/zoo_saturn/bag_2__types.v
@@ -1,7 +1,7 @@
 Require Import zoo.prelude.
 Require Import zoo.language.typeclasses.
 Require Import zoo.language.notations.
-Require Export zoo_saturn.spmc_queue.
+Require Export zoo_saturn.queue_spmc.
 Require Export zoo_std.domain.
 Require Import zoo.options.
 
