theories/zoo_saturn/queue_spmc__code.v
@@ -1,0 +1,82 @@
+Require Import zoo.prelude.
+Require Import zoo.language.typeclasses.
+Require Import zoo.language.notations.
+Require Import zoo_std.domain.
+Require Import zoo.options.
+
+Notation "'queue_spmc٠Null'" := (
+  in_type "zoo_saturn.queue_spmc.node" 0
+)(in custom zoo_tag
+).
+Notation "'queue_spmc٠Node'" := (
+  in_type "zoo_saturn.queue_spmc.node" 1
+)(in custom zoo_tag
+).
+
+Notation "'queue_spmc٠next'" := (
+  in_type "zoo_saturn.queue_spmc.node.Node" 0
+)(in custom zoo_field
+).
+Notation "'queue_spmc٠data'" := (
+  in_type "zoo_saturn.queue_spmc.node.Node" 1
+)(in custom zoo_field
+).
+
+Notation "'queue_spmc٠front'" := (
+  in_type "zoo_saturn.queue_spmc.t" 0
+)(in custom zoo_field
+).
+Notation "'queue_spmc٠back'" := (
+  in_type "zoo_saturn.queue_spmc.t" 1
+)(in custom zoo_field
+).
+
+Definition queue_spmc٠create : val :=
+  𝗳𝘂𝗻 ⎽ ->
+    𝗹𝗲𝘁 "front" =
+      ‘queue_spmc٠Node{ §queue_spmc٠Null, () }
+    𝗶𝗻
+    { "front", "front" }.
+
+Definition queue_spmc٠is_empty : val :=
+  𝗳𝘂𝗻 "t" ->
+    𝗺𝗮𝘁𝗰𝗵 "t".{queue_spmc٠front} 𝘄𝗶𝘁𝗵
+    | queue_spmc٠Node ⎽ ⎽ 𝗮𝘀 "front_r" ->
+        "front_r".{queue_spmc٠next} == §queue_spmc٠Null
+    𝗲𝗻𝗱.
+
+Definition queue_spmc٠push : val :=
+  𝗳𝘂𝗻 "t" "v" ->
+    𝗺𝗮𝘁𝗰𝗵
+      ‘queue_spmc٠Node{ §queue_spmc٠Null, "v" }
+    𝘄𝗶𝘁𝗵
+    | queue_spmc٠Node ⎽ ⎽ 𝗮𝘀 "new_back" ->
+        𝗺𝗮𝘁𝗰𝗵 "t".{queue_spmc٠back} 𝘄𝗶𝘁𝗵
+        | queue_spmc٠Node ⎽ ⎽ 𝗮𝘀 "back_r" ->
+            "back_r" <-{queue_spmc٠next} "new_back" ⍮
+            "t" <-{queue_spmc٠back} "new_back"
+        𝗲𝗻𝗱
+    𝗲𝗻𝗱.
+
+Definition queue_spmc٠pop : val :=
+  𝗿𝗲𝗰 "pop" "t" ->
+    𝗺𝗮𝘁𝗰𝗵 "t".{queue_spmc٠front} 𝘄𝗶𝘁𝗵
+    | queue_spmc٠Node ⎽ ⎽ 𝗮𝘀 "front" ->
+        𝗹𝗲𝘁 "front_r" = "front" 𝗶𝗻
+        𝗺𝗮𝘁𝗰𝗵 "front_r".{queue_spmc٠next} 𝘄𝗶𝘁𝗵
+        | queue_spmc٠Null ->
+            §None
+        | queue_spmc٠Node ⎽ ⎽ 𝗮𝘀 "new_front" ->
+            𝗹𝗲𝘁 "new_front_r" = "new_front" 𝗶𝗻
+            𝗶𝗳
+              𝗰𝗮𝘀 "t".[queue_spmc٠front] "front" "new_front"
+            𝘁𝗵𝗲𝗻 (
+              𝗹𝗲𝘁 "v" = "new_front_r".{queue_spmc٠data} 𝗶𝗻
+              "new_front_r" <-{queue_spmc٠data} () ⍮
+              ‘Some( "v" )
+            ) 𝗲𝗹𝘀𝗲 (
+              domain٠yield () ⍮
+              "pop" "t"
+            )
+        𝗲𝗻𝗱
+    𝗲𝗻𝗱.
