theories/zoo_saturn/queue_spmc__opaque.v
@@ -1,0 +1,6 @@
+Require Import zoo_saturn.queue_spmc__code.
+
+#[global] Opaque queue_spmc٠create.
+#[global] Opaque queue_spmc٠is_empty.
+#[global] Opaque queue_spmc٠push.
+#[global] Opaque queue_spmc٠pop.
