theories/zoo_saturn/spmc_queue__opaque.v
@@ -1,6 +1,0 @@
-Require Import zoo_saturn.spmc_queue__code.
-
-#[global] Opaque spmc_queue٠create.
-#[global] Opaque spmc_queue٠is_empty.
-#[global] Opaque spmc_queue٠push.
-#[global] Opaque spmc_queue٠pop.
